### RDF Turtle file auto-generated by "(Digdir) Excel2Turtle/Html v.3"

@prefix adms: <http://www.w3.org/ns/adms#> . 
@prefix dcat: <http://www.w3.org/ns/dcat#> . 
@prefix dct: <http://purl.org/dc/terms/> . 
@prefix rdf: <http://www.w3.org/1999/02/22-rdf-syntax-ns#> . 
@prefix schema: <http://schema.org/> . 
@prefix skos: <http://www.w3.org/2004/02/skos/core#> . 
@prefix uneskos: <http://purl.org/umu/uneskos#> . 
@prefix vcard: <http://www.w3.org/2006/vcard/ns#> . 
@prefix xkos: <http://rdf-vocabulary.ddialliance.org/xkos#> . 
@prefix xsd: <http://www.w3.org/2001/XMLSchema#> . 

<https://data.norge.no/vocabulary/audience-type>
   rdf:type skos:ConceptScheme;
   xkos:numberOfLevels "1"^^xsd:positiveInteger;
   dct:identifier "https://data.norge.no/vocabulary/audience-type"^^xsd:anyURI;
   dct:title """Målgruppetype"""@nb,
       """Målgruppetype"""@nn,
       """Audience type"""@en;
   dct:publisher <https://organization-catalog.fellesdatakatalog.digdir.no/organizations/991825827>;
   dct:description """Kontrollert vokabular med predefinerte målgruppetyper, primært ment for å brukes i forbindelse med begrepsbeskrivelser  i henhold til SKOS-AP-NO-Begrep og TBX-AP-NO."""@nb,
       """Controlled vocabulary with predefined audience types, primarily meant to be used in connection with descriptions of concepts in accordance with SKOS-AP-NO-Begrep and TBX-AP-NO."""@en;
   schema:validFrom "2022-09-01"^^xsd:date;
   uneskos:contains <https://data.norge.no/vocabulary/audience-type#public>,
       <https://data.norge.no/vocabulary/audience-type#specialist>;
   dct:modified "2023-03-16"^^xsd:date;
   dct:language <http://publications.europa.eu/resource/authority/language/NOB>,
       <http://publications.europa.eu/resource/authority/language/ENG>;
   dct:issued "2022-09-01"^^xsd:date;
   adms:status <http://publications.europa.eu/resource/authority/dataset-status/COMPLETED>;
   .
 
<https://data.norge.no/vocabulary/audience-type#public>
   rdf:type skos:Concept;
   skos:prefLabel """allmennheten"""@nb,
       """allmenta"""@nn,
       """public"""@en;
   skos:inScheme <https://data.norge.no/vocabulary/audience-type>;
   skos:topConceptOf <https://data.norge.no/vocabulary/audience-type>;
   xkos:coreContentNote """Inkluderer: målgruppe som det ikke forutsettes noe forkunnskap av, i det/de aktuelle fagområdet/fagområdene for begrepet"""@nb,
       """Includes: audience of whom there is no prior knowledge required in the subject field(s) of the concept"""@en;
   dct:identifier "https://data.norge.no/vocabulary/audience-type#public"^^xsd:anyURI;
   skos:definition """målgruppe som det ikke forutsettes noe forkunnskap av, i det/de aktuelle fagområdet/fagområdene for begrepet"""@nb,
       """audience of whom there is no prior knowledge required in the subject field(s) of the concept"""@en;
   adms:status <http://publications.europa.eu/resource/authority/concept-status/CURRENT>;
   dcat:contactPoint <https://data.norge.no/vocabulary/audience-type#Digdir>;
   dct:publisher <https://organization-catalog.fellesdatakatalog.digdir.no/organizations/991825827>;
   .
 
<https://data.norge.no/vocabulary/audience-type#specialist>
   rdf:type skos:Concept;
   skos:prefLabel """spesialist"""@nb,
       """spesialist"""@nn,
       """specialist"""@en;
   skos:inScheme <https://data.norge.no/vocabulary/audience-type>;
   xkos:coreContentNote """Inkluderer: målgruppe som det forutsettes et visst kunnskapsnivå i det/de aktuelle fagområdet/fagområdene for begrepet"""@nb,
       """Includes: audience of whom there is certain level of knowledge required in the subject field(s) of the concept"""@en;
   dct:identifier "https://data.norge.no/vocabulary/audience-type#specialist"^^xsd:anyURI;
   skos:definition """målgruppe som det forutsettes et visst kunnskapsnivå i det/de aktuelle fagområdet/fagområdene for begrepet"""@no,
       """audience of whom there is certain level of knowledge required in the subject field(s) of the concept"""@en;
   adms:status <http://publications.europa.eu/resource/authority/concept-status/CURRENT>;
   dcat:contactPoint <https://data.norge.no/vocabulary/audience-type#Digdir>;
   dct:publisher <https://organization-catalog.fellesdatakatalog.digdir.no/organizations/991825827>;
   .
 
<https://data.norge.no/vocabulary/audience-type#Digdir>
   rdf:type vcard:Organization;
   vcard:hasOrganizationName """Digitaliseringsdirektoratet (Digdir)"""@nb,
       """Norwegian Digitalisation Agency (Digdir)"""@en;
   vcard:hasEmail "informasjonsforvaltning@digdir.no"^^xsd:anyURI;
   .
 
#### End of the file, 2023-03-16 10:47:44